BigN, BigZ, BigQ: presentation via unique module with both ops and props (BACKPORT 12680)
 We use the <+ operation to regroup all known facts about BigN
 (resp BigZ, ...) in a unique module. This uses also the new ! feature
 for controling inlining. By the way, we also make sure that these
 new BigN and BigZ modules implements OrderedTypeFull and TotalOrder,
 and also contains facts about min and max (cf. GenericMinMax).

 Side effects:
 - In NSig and ZSig, specification of compare and eq_bool is now
   done with respect to Zcompare and Zeq_bool, as for other ops.
   The order <= and < are also defined via Zle and Zlt, instead
   of using compare. Min and max are axiomatized instead of being
   macros.
 - Some proofs rework in QMake
 - QOrderedType and Qminmax were in fact not compiled by make world

 Still todo: OrderedType + MinMax for BigQ, etc etc

git-svn-id: svn+ssh://scm.gforge.inria.fr/svn/coq/branches/v8.3@12733 85f007b7-540e-0410-9357-904b9bb8a0f7

theories/Numbers/Natural/BigN/NMake_gen.ml
@@ -1339,12 +1339,6 @@ let _ =
   pr "      comparenm).";
   pr "";
 
-  pr " Definition lt n m := compare n m = Lt.";
-  pr " Definition le n m := compare n m <> Gt.";
-  pr " Definition min n m := match compare n m with Gt => m | _ => n end.";
-  pr " Definition max n m := match compare n m with Lt => m | _ => n end.";
-  pr "";
-
   for i = 0 to size do
     pp " Let spec_compare_%i: forall x y," i;
     pp "    match compare_%i x y with " i;
@@ -1386,7 +1380,7 @@ let _ =
   pp "";
 
 
-  pr " Theorem spec_compare: forall x y,";
+  pr " Theorem spec_compare_aux: forall x y,";
   pr "    match compare x y with ";
   pr "      Eq => [x] = [y]";
   pr "    | Lt => [x] < [y]";
@@ -1421,6 +1415,15 @@ let _ =
   pp "  Qed.";
   pr "";
 
+  pr " Theorem spec_compare : forall x y, compare x y = Zcompare [x] [y].";
+  pa " Admitted.";
+  pp " Proof.";
+  pp " intros x y. generalize (spec_compare_aux x y); destruct compare;";
+  pp " intros; symmetry; try rewrite Zcompare_Eq_iff_eq; assumption.";
+  pp " Qed.";
+  pr "";
+
+
   pr " Definition eq_bool x y :=";
   pr "  match compare x y with";
   pr "  | Eq => true";
@@ -1428,17 +1431,42 @@ let _ =
   pr "  end.";
   pr "";
 
+  pr " Theorem spec_eq_bool : forall x y, eq_bool x y = Zeq_bool [x] [y].";
+  pa " Admitted.";
+  pp " Proof.";
+  pp " intros. unfold eq_bool, Zeq_bool. rewrite spec_compare; reflexivity.";
+  pp " Qed.";
+  pr "";
 
-  pr " Theorem spec_eq_bool: forall x y,";
+  pr " Theorem spec_eq_bool_aux: forall x y,";
   pr "    if eq_bool x y then [x] = [y] else [x] <> [y].";
   pa " Admitted.";
   pp " Proof.";
   pp " intros x y; unfold eq_bool.";
-  pp " generalize (spec_compare x y); case compare; auto with zarith.";
-  pp "  Qed.";
+  pp " generalize (spec_compare_aux x y); case compare; auto with zarith.";
+  pp " Qed.";
   pr "";
 
+  pr " Definition lt n m := [n] < [m].";
+  pr " Definition le n m := [n] <= [m].";
+  pr "";
+  pr " Definition min n m := match compare n m with Gt => m | _ => n end.";
+  pr " Definition max n m := match compare n m with Lt => m | _ => n end.";
+  pr "";
 
+  pr " Theorem spec_max : forall n m, [max n m] = Zmax [n] [m].";
+  pa " Admitted.";
+  pp " Proof.";
+  pp " intros. unfold max, Zmax. rewrite spec_compare; destruct Zcompare; reflexivity.";
+  pp " Qed.";
+  pr "";
+
+  pr " Theorem spec_min : forall n m, [min n m] = Zmin [n] [m].";
+  pa " Admitted.";
+  pp " Proof.";
+  pp " intros. unfold min, Zmin. rewrite spec_compare; destruct Zcompare; reflexivity.";
+  pp " Qed.";
+  pr "";
 
   pr " (***************************************************************)";
   pr " (*                                                             *)";
@@ -1974,12 +2002,12 @@ let _ =
   pp " assert (F1: [one] = 1).";
   pp "   exact (spec_1 w0_spec).";
   pp " intros x y. unfold div_eucl.";
-  pp " generalize (spec_eq_bool y zero). destruct eq_bool; rewrite F0.";
+  pp " generalize (spec_eq_bool_aux y zero). destruct eq_bool; rewrite F0.";
   pp " intro H. rewrite H. destruct [x]; auto.";
   pp " intro H'.";
   pp " assert (0 < [y]) by (generalize (spec_pos y); auto with zarith).";
   pp " clear H'.";
-  pp " generalize (spec_compare x y); case compare; try rewrite F0;";
+  pp " generalize (spec_compare_aux x y); case compare; try rewrite F0;";
   pp "   try rewrite F1; intros; auto with zarith.";
   pp " rewrite H0; generalize (Z_div_same [y] (Zlt_gt _ _ H))";
   pp "                        (Z_mod_same [y] (Zlt_gt _ _ H));";
@@ -2121,12 +2149,12 @@ let _ =
   pp " assert (F1: [one] = 1).";
   pp "   exact (spec_1 w0_spec).";
   pp " intros x y. unfold modulo.";
-  pp " generalize (spec_eq_bool y zero). destruct eq_bool; rewrite F0.";
+  pp " generalize (spec_eq_bool_aux y zero). destruct eq_bool; rewrite F0.";
   pp " intro H; rewrite H. destruct [x]; auto.";
   pp " intro H'.";
   pp " assert (H : 0 < [y]) by (generalize (spec_pos y); auto with zarith).";
   pp " clear H'.";
-  pp " generalize (spec_compare x y); case compare; try rewrite F0;";
+  pp " generalize (spec_compare_aux x y); case compare; try rewrite F0;";
   pp "   try rewrite F1; intros; try split; auto with zarith.";
   pp " rewrite H0; apply sym_equal; apply Z_mod_same; auto with zarith.";
   pp " apply sym_equal; apply Zmod_small; auto with zarith.";
@@ -2185,11 +2213,11 @@ let _ =
   pp " assert (F1: [zero] = 0).";
   pp "   unfold zero, w_0, to_Z; rewrite (spec_0 w0_spec); auto.";
   pp " intros a b cont p H2 H3 H4; unfold gcd_gt_body.";
-  pp " generalize (spec_compare b zero); case compare; try rewrite F1.";
+  pp " generalize (spec_compare_aux b zero); case compare; try rewrite F1.";
   pp "   intros HH; rewrite HH; apply Zis_gcd_0.";
   pp " intros HH; absurd (0 <= [b]); auto with zarith.";
   pp " case (spec_digits b); auto with zarith.";
-  pp " intros H5; generalize (spec_compare (mod_gt a b) zero); ";
+  pp " intros H5; generalize (spec_compare_aux (mod_gt a b) zero); ";
   pp "   case compare; try rewrite F1.";
   pp " intros H6; rewrite <- (Zmult_1_r [b]).";
   pp " rewrite (Z_div_mod_eq [a] [b]); auto with zarith.";
@@ -2322,7 +2350,7 @@ let _ =
   pp " intros a b.";
   pp " case (spec_digits a); intros H1 H2.";
   pp " case (spec_digits b); intros H3 H4.";
-  pp " unfold gcd; generalize (spec_compare a b); case compare.";
+  pp " unfold gcd; generalize (spec_compare_aux a b); case compare.";
   pp " intros HH; rewrite HH; apply sym_equal; apply Zis_gcd_gcd; auto.";
   pp "   apply Zis_gcd_refl.";
   pp " intros; apply trans_equal with (Zgcd [b] [a]).";
@@ -2727,7 +2755,7 @@ let _ =
   pa " Admitted.";
   pp " Proof.";
   pp " intros n x; unfold safe_shiftr;";
-  pp "    generalize (spec_compare n (Ndigits x)); case compare; intros H.";
+  pp "    generalize (spec_compare_aux n (Ndigits x)); case compare; intros H.";
   pp " apply trans_equal with (1 := spec_0 w0_spec).";
   pp " apply sym_equal; apply Zdiv_small; rewrite H.";
   pp " rewrite spec_Ndigits; exact (spec_digits x).";
@@ -3063,7 +3091,7 @@ let _ =
   pa " Admitted.";
   pp " Proof.";
   pp " intros n p x cont H1 H2; unfold safe_shiftl_aux_body.";
-  pp " generalize (spec_compare n (head0 x)); case compare; intros H.";
+  pp " generalize (spec_compare_aux n (head0 x)); case compare; intros H.";
   pp "  apply spec_shiftl; auto with zarith.";
   pp "  apply spec_shiftl; auto with zarith.";
   pp " rewrite H2.";
@@ -3131,11 +3159,11 @@ let _ =
   pa " Admitted.";
   pp " Proof.";
   pp " intros n x; unfold safe_shiftl, safe_shiftl_aux_body.";
-  pp " generalize (spec_compare n (head0 x)); case compare; intros H.";
+  pp " generalize (spec_compare_aux n (head0 x)); case compare; intros H.";
   pp "  apply spec_shiftl; auto with zarith.";
   pp "  apply spec_shiftl; auto with zarith.";
   pp " rewrite <- (spec_double_size x).";
-  pp " generalize (spec_compare n (head0 (double_size x))); case compare; intros H1.";
+  pp " generalize (spec_compare_aux n (head0 (double_size x))); case compare; intros H1.";
   pp "  apply spec_shiftl; auto with zarith.";
   pp "  apply spec_shiftl; auto with zarith.";
   pp " rewrite <- (spec_double_size (double_size x)).";
