theories/Numbers/Rational/BigQ/QMake.v
@@ -5,14 +5,19 @@
 (*    //   *      This file is distributed under the terms of the       *)
 (*         *       GNU Lesser General Public License Version 2.1        *)
 (************************************************************************)
-(*            Benjamin Gregoire, Laurent Thery, INRIA, 2007             *)
-(************************************************************************)
 
-(*i $Id$ i*)
+(** * QMake : a generic efficient implementation of rational numbers *)
+
+(** Initial authors : Benjamin Gregoire, Laurent Thery, INRIA, 2007 *)
 
 Require Import BigNumPrelude ROmega.
-Require Import QArith Qcanon Qpower.
+Require Import QArith Qcanon Qpower Qminmax.
 Require Import NSig ZSig QSig.
+
+(** We will build rationals out of an implementation of integers [ZType]
+    for numerators and an implementation of natural numbers [NType] for
+    denominators. But first we will need some glue between [NType] and
+    [ZType]. *)
 
 Module Type NType_ZType (N:NType)(Z:ZType).
  Parameter Z_of_N : N.t -> Z.t.
@@ -56,17 +61,56 @@ Module Make (N:NType)(Z:ZType)(Import NZ:NType_ZType N Z) <: QType.
 
  Notation "[ x ]" := (to_Q x).
 
+ Lemma N_to_Z_pos :
+  forall x, (N.to_Z x <> N.to_Z N.zero)%Z -> (0 < N.to_Z x)%Z.
+ Proof.
+ intros x; rewrite N.spec_0; generalize (N.spec_pos x). romega.
+ Qed.
+(*
+ Lemma if_fun_commut : forall A B (f:A->B)(b:bool) a a',
+ f (if b then a else a') = if b then f a else f a'.
+ Proof. now destruct b. Qed.
+
+ Lemma if_fun_commut' : forall A B C D (f:A->B)(b:{C}+{D}) a a',
+ f (if b then a else a') = if b then f a else f a'.
+ Proof. now destruct b. Qed.
+*)
+ Ltac destr_eqb :=
+  match goal with
+   | |- context [Z.eq_bool ?x ?y] =>
+     rewrite (Z.spec_eq_bool x y);
+     generalize (Zeq_bool_if (Z.to_Z x) (Z.to_Z y));
+     case (Zeq_bool (Z.to_Z x) (Z.to_Z y));
+     destr_eqb
+   | |- context [N.eq_bool ?x ?y] =>
+     rewrite (N.spec_eq_bool x y);
+     generalize (Zeq_bool_if (N.to_Z x) (N.to_Z y));
+     case (Zeq_bool (N.to_Z x) (N.to_Z y));
+     [ | let H:=fresh "H" in
+         try (intro H;generalize (N_to_Z_pos _ H); clear H)];
+     destr_eqb
+   | _ => idtac
+  end.
+
+ Hint Rewrite
+  Zplus_0_r Zplus_0_l Zmult_0_r Zmult_0_l Zmult_1_r Zmult_1_l
+  Z.spec_0 N.spec_0 Z.spec_1 N.spec_1 Z.spec_m1 Z.spec_opp
+  Z.spec_compare N.spec_compare
+  Z.spec_add N.spec_add Z.spec_mul N.spec_mul Z.spec_div N.spec_div
+  Z.spec_gcd N.spec_gcd Zgcd_Zabs Zgcd_1
+  spec_Z_of_N spec_Zabs_N
+ : nz.
+ Ltac nzsimpl := autorewrite with nz in *.
+
+ Ltac qsimpl := try red; unfold to_Q; simpl; intros;
+  destr_eqb; simpl; nzsimpl; intros;
+  rewrite ?Z2P_correct by auto;
+  auto.
+
  Theorem strong_spec_of_Q: forall q: Q, [of_Q q] = q.
  Proof.
- intros(x,y); destruct y; simpl; rewrite Z.spec_of_Z; auto.
- generalize (N.spec_eq_bool (N.of_N (Npos y~1)) N.zero);
-  case N.eq_bool; auto; rewrite N.spec_0.
- rewrite N.spec_of_N; discriminate.
- rewrite N.spec_of_N; auto.
- generalize (N.spec_eq_bool (N.of_N (Npos y~0)) N.zero);
-  case N.eq_bool; auto; rewrite N.spec_0.
- rewrite N.spec_of_N; discriminate.
- rewrite N.spec_of_N; auto.
+ intros(x,y); destruct y; simpl; rewrite ?Z.spec_of_Z; auto;
+  destr_eqb; now rewrite ?N.spec_0, ?N.spec_of_N.
  Qed.
 
  Theorem spec_of_Q: forall q: Q, [of_Q q] == q.
@@ -82,17 +126,17 @@ Module Make (N:NType)(Z:ZType)(Import NZ:NType_ZType N Z) <: QType.
 
  Lemma spec_0: [zero] == 0.
  Proof.
- simpl; rewrite Z.spec_0; reflexivity.
+ simpl. nzsimpl. reflexivity.
  Qed.
 
  Lemma spec_1: [one] == 1.
  Proof.
- simpl; rewrite Z.spec_1; reflexivity.
+ simpl. nzsimpl. reflexivity.
  Qed.
 
  Lemma spec_m1: [minus_one] == -(1).
  Proof.
- simpl; rewrite Z.spec_m1; reflexivity.
+ simpl. nzsimpl. reflexivity.
  Qed.
 
  Definition compare (x y: t) :=
@@ -114,83 +158,36 @@ Module Make (N:NType)(Z:ZType)(Import NZ:NType_ZType N Z) <: QType.
     end
   end.
 
- Lemma Zcompare_spec_alt :
-  forall z z', Z.compare z z' = (Z.to_Z z ?= Z.to_Z z')%Z.
- Proof.
- intros; generalize (Z.spec_compare z z'); destruct Z.compare; auto.
- intro H; rewrite H; symmetry; apply Zcompare_refl.
- Qed.
-
- Lemma Ncompare_spec_alt :
-  forall n n', N.compare n n' = (N.to_Z n ?= N.to_Z n')%Z.
- Proof.
- intros; generalize (N.spec_compare n n'); destruct N.compare; auto.
- intro H; rewrite H; symmetry; apply Zcompare_refl.
- Qed.
-
- Lemma N_to_Z2P : forall n, N.to_Z n <> 0%Z ->
-  Zpos (Z2P (N.to_Z n)) = N.to_Z n.
- Proof.
- intros; apply Z2P_correct.
- generalize (N.spec_pos n); romega.
- Qed.
-
- Hint Rewrite
-  Zplus_0_r Zplus_0_l Zmult_0_r Zmult_0_l Zmult_1_r Zmult_1_l
-  Z.spec_0 N.spec_0 Z.spec_1 N.spec_1 Z.spec_m1 Z.spec_opp
-  Zcompare_spec_alt Ncompare_spec_alt
-  Z.spec_add N.spec_add Z.spec_mul N.spec_mul
-  Z.spec_gcd N.spec_gcd Zgcd_Zabs Zgcd_1
-  spec_Z_of_N spec_Zabs_N
- : nz.
- Ltac nzsimpl := autorewrite with nz in *.
-
- Ltac destr_neq_bool := repeat
- (match goal with |- context [N.eq_bool ?x ?y] =>
-   generalize (N.spec_eq_bool x y); case N.eq_bool
-  end).
-
- Ltac destr_zeq_bool := repeat
- (match goal with |- context [Z.eq_bool ?x ?y] =>
-   generalize (Z.spec_eq_bool x y); case Z.eq_bool
-  end).
-
- Ltac simpl_ndiv := rewrite N.spec_div by (nzsimpl; romega).
- Tactic Notation "simpl_ndiv" "in" "*" :=
-   rewrite N.spec_div in * by (nzsimpl; romega).
-
- Ltac simpl_zdiv := rewrite Z.spec_div by (nzsimpl; romega).
- Tactic Notation "simpl_zdiv" "in" "*" :=
-   rewrite Z.spec_div in * by (nzsimpl; romega).
-
- Ltac qsimpl := try red; unfold to_Q; simpl; intros;
-  destr_neq_bool; destr_zeq_bool; simpl; nzsimpl; auto; intros.
-
  Theorem spec_compare: forall q1 q2, (compare q1 q2) = ([q1] ?= [q2]).
  Proof.
  intros [z1 | x1 y1] [z2 | x2 y2];
-   unfold Qcompare, compare; qsimpl; rewrite ! N_to_Z2P; auto.
+   unfold Qcompare, compare; qsimpl.
  Qed.
 
- Definition lt n m := compare n m = Lt.
- Definition le n m := compare n m <> Gt.
+ Definition lt n m := [n] < [m].
+ Definition le n m := [n] <= [m].
+
  Definition min n m := match compare n m with Gt => m | _ => n end.
  Definition max n m := match compare n m with Lt => m | _ => n end.
+
+ Lemma spec_min : forall n m, [min n m] == Qmin [n] [m].
+ Proof.
+ unfold min, Qmin, GenericMinMax.gmin. intros.
+ rewrite spec_compare; destruct Qcompare; auto with qarith.
+ Qed.
+
+ Lemma spec_max : forall n m, [max n m] == Qmax [n] [m].
+ Proof.
+ unfold max, Qmax, GenericMinMax.gmax. intros.
+ rewrite spec_compare; destruct Qcompare; auto with qarith.
+ Qed.
 
  Definition eq_bool n m :=
   match compare n m with Eq => true | _ => false end.
 
- Theorem spec_eq_bool: forall x y,
-  if eq_bool x y then [x] == [y] else ~([x] == [y]).
+ Theorem spec_eq_bool: forall x y, eq_bool x y = Qeq_bool [x] [y].
  Proof.
- intros.
- unfold eq_bool.
- rewrite spec_compare.
- generalize (Qeq_alt [x] [y]).
- destruct Qcompare.
- intros H; rewrite H; auto.
- intros H H'; rewrite H in H'; discriminate.
- intros H H'; rewrite H in H'; discriminate.
+ intros. unfold eq_bool. rewrite spec_compare. reflexivity.
  Qed.
 
  (** [check_int] : is a reduced fraction [n/d] in fact a integer ? *)
@@ -209,7 +206,7 @@ Module Make (N:NType)(Z:ZType)(Import NZ:NType_ZType N Z) <: QType.
  destr_zcompare.
  simpl. rewrite <- H; qsimpl. congruence.
  reflexivity.
- qsimpl. exfalso. generalize (N.spec_pos d); romega.
+ qsimpl. exfalso; romega.
  Qed.
 
  (** Normalisation function *)
@@ -234,12 +231,9 @@ Module Make (N:NType)(Z:ZType)(Import NZ:NType_ZType N Z) <: QType.
  (* Lt *)
  rewrite strong_spec_check_int.
  qsimpl.
- simpl_ndiv in *; nzsimpl.
- generalize (Zgcd_div_pos (Z.to_Z p) (N.to_Z q)). omega.
- simpl_ndiv in *.
- rewrite H0 in *. rewrite Zdiv_0_l in H1; elim H1; auto.
- rewrite 2 N_to_Z2P; auto.
- simpl_ndiv; simpl_zdiv; nzsimpl.
+ generalize (Zgcd_div_pos (Z.to_Z p) (N.to_Z q)). romega.
+ replace (N.to_Z q) with 0%Z in * by assumption.
+ rewrite Zdiv_0_l in *; auto with zarith.
  apply Zgcd_div_swap0; romega.
  (* Gt *)
  qsimpl.
@@ -260,20 +254,15 @@ Module Make (N:NType)(Z:ZType)(Import NZ:NType_ZType N Z) <: QType.
  nzsimpl.
  destr_zcompare; rewrite ?strong_spec_check_int.
  (* Eq *)
- simpl.
- destr_neq_bool; nzsimpl; simpl; auto.
- intros.
- rewrite N_to_Z2P; auto.
+ qsimpl.
  (* Lt *)
  qsimpl.
- rewrite N_to_Z2P; auto.
- simpl_zdiv; simpl_ndiv in *; nzsimpl.
  rewrite Zgcd_1_rel_prime.
  destruct (Z_lt_le_dec 0 (N.to_Z q)).
  apply Zis_gcd_rel_prime; auto with zarith.
  apply Zgcd_is_gcd.
  replace (N.to_Z q) with 0%Z in * by romega.
- simpl in H0; elim H0; auto.
+ rewrite Zdiv_0_l in *; romega.
  (* Gt *)
  simpl; auto with zarith.
  Qed.
@@ -286,7 +275,7 @@ Module Make (N:NType)(Z:ZType)(Import NZ:NType_ZType N Z) <: QType.
    | Qq n d => norm n d
   end.
 
- Definition Reduced x := [red x] = [x].
+ Class Reduced x := is_reduced : [red x] = [x].
 
  Theorem spec_red : forall x, [red x] == [x].
  Proof.
@@ -328,19 +317,12 @@ Module Make (N:NType)(Z:ZType)(Import NZ:NType_ZType N Z) <: QType.
 
  Theorem spec_add : forall x y, [add x y] == [x] + [y].
  Proof.
- intros [x | nx dx] [y | ny dy]; unfold Qplus; qsimpl.
- intuition.
- rewrite N_to_Z2P; auto.
- intuition.
- rewrite Pmult_1_r, N_to_Z2P; auto.
- intuition.
- rewrite Pmult_1_r, N_to_Z2P; auto.
- destruct (Zmult_integral _ _ H); intuition.
- rewrite Zpos_mult_morphism, 2 N_to_Z2P; auto.
- rewrite (Z2P_correct (N.to_Z dx * N.to_Z dy)); auto.
- apply Zmult_lt_0_compat.
-  generalize (N.spec_pos dx); romega.
-  generalize (N.spec_pos dy); romega.
+ intros [x | nx dx] [y | ny dy]; unfold Qplus; qsimpl;
+  auto with zarith.
+ rewrite Pmult_1_r, Z2P_correct; auto.
+ rewrite Pmult_1_r, Z2P_correct; auto.
+ destruct (Zmult_integral (N.to_Z dx) (N.to_Z dy)); intuition.
+ rewrite Zpos_mult_morphism, 2 Z2P_correct; auto.
  Qed.
 
  Definition add_norm (x y: t): t :=
@@ -369,25 +351,19 @@ Module Make (N:NType)(Z:ZType)(Import NZ:NType_ZType N Z) <: QType.
  Proof.
  intros x y; rewrite <- spec_add.
  destruct x; destruct y; unfold add_norm, add;
- destr_neq_bool; auto using Qeq_refl, spec_norm.
+ destr_eqb; auto using Qeq_refl, spec_norm.
  Qed.
 
- Theorem strong_spec_add_norm : forall x y : t,
-   Reduced x -> Reduced y -> Reduced (add_norm x y).
+ Instance strong_spec_add_norm x y
+   `(Reduced x, Reduced y) : Reduced (add_norm x y).
  Proof.
  unfold Reduced; intros.
  rewrite strong_spec_red.
  rewrite <- (Qred_complete [add x y]);
   [ | rewrite spec_add, spec_add_norm; apply Qeq_refl ].
  rewrite <- strong_spec_red.
- destruct x as [zx|nx dx]; destruct y as [zy|ny dy].
- simpl in *; auto.
- simpl; intros.
- destr_neq_bool; nzsimpl; simpl; auto.
- simpl; intros.
- destr_neq_bool; nzsimpl; simpl; auto.
- simpl; intros.
- destr_neq_bool; nzsimpl; simpl; auto.
+ destruct x as [zx|nx dx]; destruct y as [zy|ny dy];
+  simpl; destr_eqb; nzsimpl; simpl; auto.
  Qed.
 
  Definition opp (x: t): t :=
@@ -411,7 +387,7 @@ Module Make (N:NType)(Z:ZType)(Import NZ:NType_ZType N Z) <: QType.
  intros; rewrite strong_spec_opp; red; auto.
  Qed.
 
- Theorem strong_spec_opp_norm : forall q, Reduced q -> Reduced (opp q).
+ Instance strong_spec_opp_norm q `(Reduced q) : Reduced (opp q).
  Proof.
  unfold Reduced; intros.
  rewrite strong_spec_opp, <- H, !strong_spec_red, <- Qred_opp.
@@ -434,8 +410,8 @@ Module Make (N:NType)(Z:ZType)(Import NZ:NType_ZType N Z) <: QType.
  rewrite spec_opp; ring.
  Qed.
 
- Theorem strong_spec_sub_norm : forall x y,
-  Reduced x -> Reduced y -> Reduced (sub_norm x y).
+ Instance strong_spec_sub_norm x y
+  `(Reduced x, Reduced y) : Reduced (sub_norm x y).
  Proof.
  intros.
  unfold sub_norm.
@@ -454,24 +430,23 @@ Module Make (N:NType)(Z:ZType)(Import NZ:NType_ZType N Z) <: QType.
  Theorem spec_mul : forall x y, [mul x y] == [x] * [y].
  Proof.
  intros [x | nx dx] [y | ny dy]; unfold Qmult; simpl; qsimpl.
- rewrite Pmult_1_r, N_to_Z2P; auto.
- destruct (Zmult_integral _ _ H1); intuition.
- rewrite H0 in H1; elim H1; auto.
- rewrite H0 in H1; elim H1; auto.
- rewrite H in H1; nzsimpl; elim H1; auto.
- rewrite Zpos_mult_morphism, 2 N_to_Z2P; auto.
- rewrite (Z2P_correct (N.to_Z dx * N.to_Z dy)); auto.
- apply Zmult_lt_0_compat.
-  generalize (N.spec_pos dx); omega.
-  generalize (N.spec_pos dy); omega.
+ rewrite Pmult_1_r, Z2P_correct; auto.
+ destruct (Zmult_integral (N.to_Z dx) (N.to_Z dy)); intuition.
+ rewrite H0 in H1; auto with zarith.
+ rewrite H0 in H1; auto with zarith.
+ rewrite H in H1; nzsimpl; auto with zarith.
+ rewrite Zpos_mult_morphism, 2 Z2P_correct; auto.
  Qed.
 
- Lemma norm_denum : forall n d,
-  [if N.eq_bool d N.one then Qz n else Qq n d] == [Qq n d].
+ Definition norm_denum n d :=
+  if N.eq_bool d N.one then Qz n else Qq n d.
+
+ Lemma spec_norm_denum : forall n d,
+  [norm_denum n d] == [Qq n d].
  Proof.
- intros; simpl; qsimpl.
- rewrite H0 in H; discriminate.
- rewrite N_to_Z2P, H0; auto with zarith.
+ unfold norm_denum; intros; simpl; qsimpl.
+ congruence.
+ rewrite H0 in *; auto with zarith.
  Qed.
 
  Definition irred n d :=
@@ -499,10 +474,10 @@ Module Make (N:NType)(Z:ZType)(Import NZ:NType_ZType N Z) <: QType.
  exists (Zgcd (Z.to_Z n) (N.to_Z d)).
  simpl.
  split.
- simpl_zdiv; nzsimpl.
+ nzsimpl.
  destruct (Zgcd_is_gcd (Z.to_Z n) (N.to_Z d)).
  rewrite Zmult_comm; symmetry; apply Zdivide_Zdiv_eq; auto with zarith.
- simpl_ndiv; nzsimpl.
+ nzsimpl.
  destruct (Zgcd_is_gcd (Z.to_Z n) (N.to_Z d)).
  rewrite Zmult_comm; symmetry; apply Zdivide_Zdiv_eq; auto with zarith.
  Qed.
@@ -516,10 +491,10 @@ Module Make (N:NType)(Z:ZType)(Import NZ:NType_ZType N Z) <: QType.
  nzsimpl; intros.
  destr_zcompare; auto.
  simpl.
- simpl_ndiv; nzsimpl.
+ nzsimpl.
  rewrite H, Zdiv_0_l; auto.
  nzsimpl; destr_zcompare; simpl; auto.
- simpl_ndiv; nzsimpl.
+ nzsimpl.
  intros.
  generalize (N.spec_pos d); intros.
  destruct (N.to_Z d); auto.
@@ -542,7 +517,7 @@ Module Make (N:NType)(Z:ZType)(Import NZ:NType_ZType N Z) <: QType.
  apply (Zgcd_inv_0_r (Z.to_Z n)).
  generalize (Zgcd_is_pos (Z.to_Z n) (N.to_Z d)); romega.
 
- simpl_ndiv; simpl_zdiv; nzsimpl.
+ nzsimpl.
  rewrite Zgcd_1_rel_prime.
  apply Zis_gcd_rel_prime.
  generalize (N.spec_pos d); romega.
@@ -558,7 +533,7 @@ Module Make (N:NType)(Z:ZType)(Import NZ:NType_ZType N Z) <: QType.
       | Gt =>
         let z := Z.div z (Z_of_N gcd) in
         let d := N.div d gcd in
-        if N.eq_bool d N.one then Qz (Z.mul z n) else Qq (Z.mul z n) d
+        norm_denum (Z.mul z n) d
       | _  => Qq (Z.mul z n) d
     end.
 
@@ -570,69 +545,61 @@ Module Make (N:NType)(Z:ZType)(Import NZ:NType_ZType N Z) <: QType.
  | Qq nx dx, Qq ny dy =>
     let (nx, dy) := irred nx dy in
     let (ny, dx) := irred ny dx in
-    let d := N.mul dx dy in
-    if N.eq_bool d N.one then Qz (Z.mul ny nx) else Qq (Z.mul ny nx) d
+    norm_denum (Z.mul ny nx) (N.mul dx dy)
  end.
 
  Lemma spec_mul_norm_Qz_Qq : forall z n d,
    [mul_norm_Qz_Qq z n d] == [Qq (Z.mul z n) d].
  Proof.
  intros z n d; unfold mul_norm_Qz_Qq; nzsimpl; rewrite Zcompare_gt.
- destr_zeq_bool; intros Hz; nzsimpl.
+ destr_eqb; nzsimpl; intros Hz.
  qsimpl; rewrite Hz; auto.
- assert (Hd := N.spec_pos d).
- destruct Z_le_gt_dec.
+ destruct Z_le_gt_dec; intros.
  qsimpl.
- rewrite norm_denum.
+ rewrite spec_norm_denum.
  qsimpl.
- simpl_ndiv in *; nzsimpl.
- rewrite (Zdiv_gcd_zero _ _ H0 H) in z0; discriminate.
- simpl_ndiv in *; nzsimpl.
- rewrite H, Zdiv_0_l in H0; elim H0; auto.
- rewrite 2 N_to_Z2P; auto.
- simpl_ndiv; simpl_zdiv; nzsimpl.
- rewrite (Zmult_comm (Z.to_Z z)), <- 2 Zmult_assoc.
- rewrite <- Zgcd_div_swap0; auto with zarith; ring.
+ rewrite Zdiv_gcd_zero in z0; auto with zarith.
+ rewrite H in *. rewrite Zdiv_0_l in *; discriminate.
+ rewrite <- Zmult_assoc, (Zmult_comm (Z.to_Z n)), Zmult_assoc.
+ rewrite Zgcd_div_swap0; try romega.
+ ring.
  Qed.
 
- Lemma strong_spec_mul_norm_Qz_Qq : forall z n d,
-   Reduced (Qq n d) -> Reduced (mul_norm_Qz_Qq z n d).
+ Instance strong_spec_mul_norm_Qz_Qq z n d
+   `(Reduced (Qq n d)) : Reduced (mul_norm_Qz_Qq z n d).
  Proof.
  unfold Reduced; intros z n d.
  rewrite 2 strong_spec_red, 2 Qred_iff.
  simpl; nzsimpl.
- destr_neq_bool; intros Hd H; simpl in *; nzsimpl.
+ destr_eqb; intros Hd H; simpl in *; nzsimpl.
 
  unfold mul_norm_Qz_Qq; nzsimpl; rewrite Zcompare_gt.
- destr_zeq_bool; intros Hz; simpl; nzsimpl; simpl; auto.
+ destr_eqb; intros Hz; simpl; nzsimpl; simpl; auto.
  destruct Z_le_gt_dec.
  simpl; nzsimpl.
- destr_neq_bool; simpl; nzsimpl; auto.
- intros H'; elim H'; auto.
- destr_neq_bool; simpl; nzsimpl.
- simpl_ndiv; nzsimpl; rewrite Hd, Zdiv_0_l; discriminate.
+ destr_eqb; simpl; nzsimpl; auto with zarith.
+ unfold norm_denum. destr_eqb; simpl; nzsimpl.
+ rewrite Hd, Zdiv_0_l; discriminate.
  intros _.
- destr_neq_bool; simpl; nzsimpl; auto.
- simpl_ndiv; nzsimpl; rewrite Hd, Zdiv_0_l; intro H'; elim H'; auto.
+ destr_eqb; simpl; nzsimpl; auto.
+ nzsimpl; rewrite Hd, Zdiv_0_l; auto with zarith.
 
- rewrite N_to_Z2P in H; auto.
+ rewrite Z2P_correct in H; auto.
  unfold mul_norm_Qz_Qq; nzsimpl; rewrite Zcompare_gt.
- destr_zeq_bool; intros Hz; simpl; nzsimpl; simpl; auto.
+ destr_eqb; intros Hz; simpl; nzsimpl; simpl; auto.
  destruct Z_le_gt_dec as [H'|H'].
  simpl; nzsimpl.
- destr_neq_bool; simpl; nzsimpl; auto.
+ destr_eqb; simpl; nzsimpl; auto.
  intros.
- rewrite N_to_Z2P; auto.
+ rewrite Z2P_correct; auto.
  apply Zgcd_mult_rel_prime; auto.
   generalize (Zgcd_inv_0_l (Z.to_Z z) (N.to_Z d))
     (Zgcd_is_pos (Z.to_Z z) (N.to_Z d)); romega.
- destr_neq_bool; simpl; nzsimpl; auto.
- simpl_ndiv; simpl_zdiv; nzsimpl.
- intros.
- destr_neq_bool; simpl; nzsimpl; auto.
- simpl_ndiv in *; nzsimpl.
- intros.
- rewrite Z2P_correct.
+ destr_eqb; simpl; nzsimpl; auto.
+ unfold norm_denum.
+ destr_eqb; nzsimpl; simpl; destr_eqb; simpl; auto.
+ intros; nzsimpl.
+ rewrite Z2P_correct; auto.
  apply Zgcd_mult_rel_prime.
  rewrite Zgcd_1_rel_prime.
  apply Zis_gcd_rel_prime.
@@ -648,9 +615,6 @@ Module Make (N:NType)(Z:ZType)(Import NZ:NType_ZType N Z) <: QType.
  rewrite <- Huv; rewrite Hd0 at 2; ring.
  rewrite Hd0 at 1.
  symmetry; apply Z_div_mult_full; auto with zarith.
- apply Zgcd_div_pos.
- generalize (N.spec_pos d); romega.
- generalize (Zgcd_is_pos (Z.to_Z z) (N.to_Z d)); romega.
  Qed.
 
  Theorem spec_mul_norm : forall x y, [mul_norm x y] == [x] * [y].
@@ -668,30 +632,24 @@ Module Make (N:NType)(Z:ZType)(Import NZ:NType_ZType N Z) <: QType.
  assert (Hz':= spec_irred_zero ny dx).
  destruct irred as (n1,d1); destruct irred as (n2,d2).
  simpl snd in *; destruct Hg as [Hg1 Hg2]; destruct Hg' as [Hg1' Hg2'].
- rewrite norm_denum.
+ rewrite spec_norm_denum.
  qsimpl.
 
- elim H; destruct (Zmult_integral _ _ H0) as [Eq|Eq].
- rewrite <- Hz' in Eq; rewrite Eq; simpl; auto.
- rewrite <- Hz in Eq; rewrite Eq; nzsimpl; auto.
+ destruct (Zmult_integral _ _ H0) as [Eq|Eq].
+ rewrite Eq in *; simpl in *.
+ rewrite <- Hg2' in *; auto with zarith.
+ rewrite Eq in *; simpl in *.
+ rewrite <- Hg2 in *; auto with zarith.
 
- elim H0; destruct (Zmult_integral _ _ H) as [Eq|Eq].
- rewrite Hz' in Eq; rewrite Eq; simpl; auto.
- rewrite Hz in Eq; rewrite Eq; nzsimpl; auto.
+ destruct (Zmult_integral _ _ H) as [Eq|Eq].
+ rewrite Hz' in Eq; rewrite Eq in *; auto with zarith.
+ rewrite Hz in Eq; rewrite Eq in *; auto with zarith.
 
- rewrite 2 Z2P_correct.
  rewrite <- Hg1, <- Hg2, <- Hg1', <- Hg2'; ring.
-
- assert (0 <= N.to_Z d2 * N.to_Z d1)%Z
-  by (apply Zmult_le_0_compat; apply N.spec_pos).
- romega.
- assert (0 <= N.to_Z dx * N.to_Z dy)%Z
-  by (apply Zmult_le_0_compat; apply N.spec_pos).
- romega.
  Qed.
 
- Theorem strong_spec_mul_norm : forall x y,
-  Reduced x -> Reduced y -> Reduced (mul_norm x y).
+ Instance strong_spec_mul_norm x y
+  `(Reduced x, Reduced y) : Reduced (mul_norm x y).
  Proof.
  unfold Reduced; intros.
  rewrite strong_spec_red, Qred_iff.
@@ -710,18 +668,21 @@ Module Make (N:NType)(Z:ZType)(Import NZ:NType_ZType N Z) <: QType.
  assert (Hgc' := strong_spec_irred ny dx).
  destruct irred as (n1,d1); destruct irred as (n2,d2).
  simpl snd in *; destruct Hg as [Hg1 Hg2]; destruct Hg' as [Hg1' Hg2'].
- destr_neq_bool; simpl; nzsimpl; intros; auto.
- destr_neq_bool; simpl; nzsimpl; intros; auto.
+
+ unfold norm_denum; qsimpl.
+
+ assert (NEQ : N.to_Z dy <> 0%Z) by
+  (rewrite Hz; intros EQ; rewrite EQ in *; romega).
+ specialize (Hgc NEQ).
+
+ assert (NEQ' : N.to_Z dx <> 0%Z) by
+  (rewrite Hz'; intro EQ; rewrite EQ in *; romega).
+ specialize (Hgc' NEQ').
 
  revert H H0.
  rewrite 2 strong_spec_red, 2 Qred_iff; simpl.
- destr_neq_bool; simpl; nzsimpl; intros.
- rewrite Hz in H; rewrite H in H2; nzsimpl; elim H2; auto.
- rewrite Hz' in H0; rewrite H0 in H2; nzsimpl; elim H2; auto.
- rewrite Hz in H; rewrite H in H2; nzsimpl; elim H2; auto.
-
- rewrite N_to_Z2P in *; auto.
- rewrite Z2P_correct.
+ destr_eqb; simpl; nzsimpl; try romega; intros.
+ rewrite Z2P_correct in *; auto.
 
  apply Zgcd_mult_rel_prime; rewrite Zgcd_comm;
   apply Zgcd_mult_rel_prime; rewrite Zgcd_comm; auto.
@@ -737,10 +698,6 @@ Module Make (N:NType)(Z:ZType)(Import NZ:NType_ZType N Z) <: QType.
  destruct (rel_prime_bezout _ _ H3) as [u v Huv].
  apply Bezout_intro with (u*g)%Z (v*g')%Z.
  rewrite <- Huv, <- Hg2', <- Hg1. ring.
-
- assert (0 <= N.to_Z d2 * N.to_Z d1)%Z.
-  apply Zmult_le_0_compat; apply N.spec_pos.
- romega.
  Qed.
 
  Definition inv (x: t): t :=
@@ -764,13 +721,13 @@ Module Make (N:NType)(Z:ZType)(Import NZ:NType_ZType N Z) <: QType.
  destruct x as [ z | n d ].
  (* Qz z *)
  simpl.
- rewrite Zcompare_spec_alt; destr_zcompare.
+ rewrite Z.spec_compare; destr_zcompare.
  (* 0 = z *)
  rewrite <- H.
  simpl; nzsimpl; compute; auto.
  (* 0 < z *)
  simpl.
- destr_neq_bool; nzsimpl; [ intros; rewrite Zabs_eq in *; romega | intros _ ].
+ destr_eqb; nzsimpl; [ intros; rewrite Zabs_eq in *; romega | intros _ ].
  set (z':=Z.to_Z z) in *; clearbody z'.
  red; simpl.
  rewrite Zabs_eq by romega.
@@ -778,7 +735,7 @@ Module Make (N:NType)(Z:ZType)(Import NZ:NType_ZType N Z) <: QType.
  unfold Qinv; simpl; destruct z'; simpl; auto; discriminate.
  (* 0 > z *)
  simpl.
- destr_neq_bool; nzsimpl; [ intros; rewrite Zabs_non_eq in *; romega | intros _ ].
+ destr_eqb; nzsimpl; [ intros; rewrite Zabs_non_eq in *; romega | intros _ ].
  set (z':=Z.to_Z z) in *; clearbody z'.
  red; simpl.
  rewrite Zabs_non_eq by romega.
@@ -786,14 +743,14 @@ Module Make (N:NType)(Z:ZType)(Import NZ:NType_ZType N Z) <: QType.
  unfold Qinv; simpl; destruct z'; simpl; auto; discriminate.
  (* Qq n d *)
  simpl.
- rewrite Zcompare_spec_alt; destr_zcompare.
+ rewrite Z.spec_compare; destr_zcompare.
  (* 0 = n *)
  rewrite <- H.
  simpl; nzsimpl.
- destr_neq_bool; intros; compute; auto.
+ destr_eqb; intros; compute; auto.
  (* 0 < n *)
  simpl.
- destr_neq_bool; nzsimpl; intros.
+ destr_eqb; nzsimpl; intros.
  intros; rewrite Zabs_eq in *; romega.
  intros; rewrite Zabs_eq in *; romega.
  clear H1.
@@ -805,10 +762,10 @@ Module Make (N:NType)(Z:ZType)(Import NZ:NType_ZType N Z) <: QType.
  red; simpl.
  rewrite Z2P_correct by auto.
  unfold Qinv; simpl; destruct n'; simpl; auto; try discriminate.
- rewrite Zpos_mult_morphism, N_to_Z2P; auto.
+ rewrite Zpos_mult_morphism, Z2P_correct; auto.
  (* 0 > n *)
  simpl.
- destr_neq_bool; nzsimpl; intros.
+ destr_eqb; nzsimpl; intros.
  intros; rewrite Zabs_non_eq in *; romega.
  intros; rewrite Zabs_non_eq in *; romega.
  clear H1.
@@ -820,7 +777,7 @@ Module Make (N:NType)(Z:ZType)(Import NZ:NType_ZType N Z) <: QType.
  rewrite Z2P_correct by romega.
  unfold Qinv; simpl; destruct n'; simpl; auto; try discriminate.
  assert (T : forall x, Zneg x = Zopp (Zpos x)) by auto.
- rewrite T, Zpos_mult_morphism, N_to_Z2P; auto; ring.
+ rewrite T, Zpos_mult_morphism, Z2P_correct; auto; ring.
  Qed.
 
  Definition inv_norm (x: t): t :=
@@ -855,28 +812,28 @@ Module Make (N:NType)(Z:ZType)(Import NZ:NType_ZType N Z) <: QType.
  destruct x as [ z | n d ].
  (* Qz z *)
  simpl.
- rewrite Zcompare_spec_alt; destr_zcompare; auto with qarith.
+ rewrite Z.spec_compare; destr_zcompare; auto with qarith.
  (* Qq n d *)
- simpl; nzsimpl; destr_neq_bool.
+ simpl; nzsimpl; destr_eqb.
  destr_zcompare; simpl; auto with qarith.
- destr_neq_bool; nzsimpl; auto with qarith.
+ destr_eqb; nzsimpl; auto with qarith.
  intros _ Hd; rewrite Hd; auto with qarith.
- destr_neq_bool; nzsimpl; auto with qarith.
+ destr_eqb; nzsimpl; auto with qarith.
  intros _ Hd; rewrite Hd; auto with qarith.
  (* 0 < n *)
  destr_zcompare; auto with qarith.
  destr_zcompare; nzsimpl; simpl; auto with qarith; intros.
- destr_neq_bool; nzsimpl; [ intros; rewrite Zabs_eq in *; romega | intros _ ].
+ destr_eqb; nzsimpl; [ intros; rewrite Zabs_eq in *; romega | intros _ ].
  rewrite H0; auto with qarith.
  romega.
  (* 0 > n *)
  destr_zcompare; nzsimpl; simpl; auto with qarith.
- destr_neq_bool; nzsimpl; [ intros; rewrite Zabs_non_eq in *; romega | intros _ ].
+ destr_eqb; nzsimpl; [ intros; rewrite Zabs_non_eq in *; romega | intros _ ].
  rewrite H0; auto with qarith.
  romega.
  Qed.
 
- Theorem strong_spec_inv_norm : forall x, Reduced x -> Reduced (inv_norm x).
+ Instance strong_spec_inv_norm x `(Reduced x) : Reduced (inv_norm x).
  Proof.
  unfold Reduced.
  intros.
@@ -885,42 +842,40 @@ Module Make (N:NType)(Z:ZType)(Import NZ:NType_ZType N Z) <: QType.
  simpl; nzsimpl.
  rewrite strong_spec_red, Qred_iff.
  destr_zcompare; simpl; nzsimpl; auto.
- destr_neq_bool; nzsimpl; simpl; auto.
- destr_neq_bool; nzsimpl; simpl; auto.
+ destr_eqb; nzsimpl; simpl; auto.
+ destr_eqb; nzsimpl; simpl; auto.
  (* Qq n d *)
  rewrite strong_spec_red, Qred_iff in H; revert H.
  simpl; nzsimpl.
- destr_neq_bool; nzsimpl; auto with qarith.
+ destr_eqb; nzsimpl; auto with qarith.
  destr_zcompare; simpl; nzsimpl; auto; intros.
  (* 0 < n *)
  destr_zcompare; simpl; nzsimpl; auto.
- destr_neq_bool; nzsimpl; simpl; auto.
+ destr_eqb; nzsimpl; simpl; auto.
  rewrite Zabs_eq; romega.
  intros _.
  rewrite strong_spec_norm; simpl; nzsimpl.
- destr_neq_bool; nzsimpl.
+ destr_eqb; nzsimpl.
  rewrite Zabs_eq; romega.
  intros _.
  rewrite Qred_iff.
  simpl.
  rewrite Zabs_eq; auto with zarith.
- rewrite N_to_Z2P in *; auto.
- rewrite Z2P_correct; auto with zarith.
+ rewrite Z2P_correct in *; auto.
  rewrite Zgcd_comm; auto.
  (* 0 > n *)
- destr_neq_bool; nzsimpl; simpl; auto; intros.
+ destr_eqb; nzsimpl; simpl; auto; intros.
  destr_zcompare; simpl; nzsimpl; auto.
- destr_neq_bool; nzsimpl.
+ destr_eqb; nzsimpl.
  rewrite Zabs_non_eq; romega.
  intros _.
  rewrite strong_spec_norm; simpl; nzsimpl.
- destr_neq_bool; nzsimpl.
+ destr_eqb; nzsimpl.
  rewrite Zabs_non_eq; romega.
  intros _.
  rewrite Qred_iff.
  simpl.
- rewrite N_to_Z2P in *; auto.
- rewrite Z2P_correct; auto with zarith.
+ rewrite Z2P_correct in *; auto.
  intros.
  rewrite Zgcd_comm, Zgcd_Zabs, Zgcd_comm.
  apply Zis_gcd_gcd; auto with zarith.
@@ -949,8 +904,8 @@ Module Make (N:NType)(Z:ZType)(Import NZ:NType_ZType N Z) <: QType.
  apply spec_inv_norm; auto.
  Qed.
 
- Theorem strong_spec_div_norm : forall x y,
-   Reduced x -> Reduced y -> Reduced (div_norm x y).
+ Instance strong_spec_div_norm x y
+   `(Reduced x, Reduced y) : Reduced (div_norm x y).
  Proof.
  intros; unfold div_norm.
  apply strong_spec_mul_norm; auto.
@@ -968,14 +923,12 @@ Module Make (N:NType)(Z:ZType)(Import NZ:NType_ZType N Z) <: QType.
  destruct x as [ z | n d ].
  simpl; rewrite Z.spec_square; red; auto.
  simpl.
- destr_neq_bool; nzsimpl; intros.
+ destr_eqb; nzsimpl; intros.
  apply Qeq_refl.
  rewrite N.spec_square in *; nzsimpl.
- contradict H; elim (Zmult_integral _ _ H0); auto.
+ elim (Zmult_integral _ _ H0); romega.
  rewrite N.spec_square in *; nzsimpl.
- rewrite H in H0; simpl in H0; elim H0; auto.
- assert (0 < N.to_Z d)%Z by (generalize (N.spec_pos d); romega).
- clear H H0.
+ rewrite H in H0; romega.
  rewrite Z.spec_square, N.spec_square.
  red; simpl.
  rewrite Zpos_mult_morphism; rewrite !Z2P_correct; auto.
@@ -1000,37 +953,35 @@ Module Make (N:NType)(Z:ZType)(Import NZ:NType_ZType N Z) <: QType.
  (* Qq *)
  simpl.
  rewrite Z.spec_power_pos.
- destr_neq_bool; nzsimpl; intros.
+ destr_eqb; nzsimpl; intros.
  apply Qeq_sym; apply Qpower_positive_0.
  rewrite N.spec_power_pos in *.
- assert (0 < N.to_Z d ^ ' p)%Z.
-  apply Zpower_gt_0; auto with zarith.
-  generalize (N.spec_pos d); romega.
+ assert (0 < N.to_Z d ^ ' p)%Z by
+  (apply Zpower_gt_0; auto with zarith).
  romega.
  rewrite N.spec_power_pos, H in *.
- rewrite Zpower_0_l in H0; [ elim H0; auto | discriminate ].
+ rewrite Zpower_0_l in H0; [romega|discriminate].
  rewrite Qpower_decomp.
  red; simpl; do 3 f_equal.
  rewrite Z2P_correct by (generalize (N.spec_pos d); romega).
  rewrite N.spec_power_pos. auto.
  Qed.
 
- Theorem strong_spec_power_pos : forall x p,
-  Reduced x -> Reduced (power_pos x p).
+ Instance strong_spec_power_pos x p `(Reduced x) : Reduced (power_pos x p).
  Proof.
  destruct x as [z | n d]; simpl; intros.
  red; simpl; auto.
  red; simpl; intros.
  rewrite strong_spec_norm; simpl.
- destr_neq_bool; nzsimpl; intros.
+ destr_eqb; nzsimpl; intros.
  simpl; auto.
  rewrite Qred_iff.
  revert H.
  unfold Reduced; rewrite strong_spec_red, Qred_iff; simpl.
- destr_neq_bool; nzsimpl; simpl; intros.
+ destr_eqb; nzsimpl; simpl; intros.
  rewrite N.spec_power_pos in H0.
- elim H0; rewrite H; rewrite Zpower_0_l; auto; discriminate.
- rewrite N_to_Z2P in *; auto.
+ rewrite H, Zpower_0_l in *; [romega|discriminate].
+ rewrite Z2P_correct in *; auto.
  rewrite N.spec_power_pos, Z.spec_power_pos; auto.
  rewrite Zgcd_1_rel_prime in *.
  apply rel_prime_Zpower; auto with zarith.
@@ -1068,8 +1019,8 @@ Module Make (N:NType)(Z:ZType)(Import NZ:NType_ZType N Z) <: QType.
  rewrite spec_inv_norm, spec_power_pos; apply Qeq_refl.
  Qed.
 
- Theorem strong_spec_power_norm : forall x z,
-   Reduced x -> Reduced (power_norm x z).
+ Instance strong_spec_power_norm x z
+   `(Reduced x) : Reduced (power_norm x z).
  Proof.
  destruct z; simpl.
  intros _; unfold Reduced; rewrite strong_spec_red.
@@ -1096,7 +1047,7 @@ Module Make (N:NType)(Z:ZType)(Import NZ:NType_ZType N Z) <: QType.
  unfold of_Qc; rewrite strong_spec_of_Q; auto.
  Qed.
 
- Lemma strong_spec_of_Qc_bis : forall q, Reduced (of_Qc q).
+ Instance strong_spec_of_Qc_bis q : Reduced (of_Qc q).
  Proof.
  intros; red; rewrite strong_spec_red, strong_spec_of_Qc.
  destruct q; simpl; auto.
@@ -1297,7 +1248,7 @@ Module Make (N:NType)(Z:ZType)(Import NZ:NType_ZType N Z) <: QType.
  unfold Qcinv, Q2Qc, this; rewrite Qred_correct; auto with qarith.
  Qed.
 
- Theorem spec_squarec x: [[square x]] =  [[x]]^2.
+ Theorem spec_squarec x: [[square x]] = [[x]]^2.
  Proof.
  intros x; unfold to_Qc.
  apply trans_equal with (!! ([x]^2)).
